src/ssa/opsem_inst.v
@@ -26,7 +26,6 @@ Require Import Floats.
 Require Import AST.
 Require Import Maps.
 Require Import opsem.
-Require Import opsem_props.
 Require Import dopsem.
 
 (************** Instantiate GVs ******************)
@@ -450,7 +449,7 @@ Global Opaque NDGVs.instantiate_gvs NDGVs.inhabited NDGVs.cgv2gvs NDGVs.gv2gvs
   DGVs.instantiate_gvs DGVs.inhabited DGVs.cgv2gvs DGVs.gv2gvs
   DGVs.lift_op1 DGVs.lift_op2 DGVs.t.
 
-Fixpoint instantiate_locals (lc1 : DOS.GVsMap) (lc2 : NDOS.GVsMap) : Prop :=
+Fixpoint instantiate_locals (lc1 : DOS.Sem.GVsMap) (lc2 : NDOS.GVsMap): Prop :=
 match lc1, lc2 with
 | nil, nil => True
 | (id1,gvs1)::lc1', (id2,gvs2)::lc2' => 
@@ -458,24 +457,24 @@ match lc1, lc2 with
 | _, _ => False
 end.
 
-Definition instantiate_EC (ec1 : DOS.ExecutionContext) 
+Definition instantiate_EC (ec1 : DOS.Sem.ExecutionContext) 
   (ec2 : NDOS.ExecutionContext) : Prop :=
 match ec1, ec2 with
-| DOS.mkEC f1 b1 cs1 tmn1 lc1 als1, NDOS.mkEC f2 b2 cs2 tmn2 lc2 als2 =>
+| DOS.Sem.mkEC f1 b1 cs1 tmn1 lc1 als1, NDOS.mkEC f2 b2 cs2 tmn2 lc2 als2 =>
     f1 = f2 /\ b1 = b2 /\ cs1 = cs2 /\ tmn1 = tmn2 /\
     instantiate_locals lc1 lc2 /\ als1 = als2
 end.
 
-Fixpoint instantiate_ECs (ecs1 : DOS.ECStack) (ecs2 : NDOS.ECStack) : Prop :=
+Fixpoint instantiate_ECs (ecs1 : DOS.Sem.ECStack) (ecs2 : NDOS.ECStack) : Prop :=
 match ecs1, ecs2 with
 | nil, nil => True
 | ec1::ecs1', ec2::ecs2' => instantiate_EC ec1 ec2 /\ instantiate_ECs ecs1' ecs2'
 | _, _ => False
 end.
 
-Definition instantiate_State (st1 : DOS.State) (st2 : NDOS.State) : Prop :=
+Definition instantiate_State (st1 : DOS.Sem.State) (st2 : NDOS.State) : Prop :=
 match st1, st2 with
-| DOS.mkState s1 td1 ps1 ecs1 gl1 fs1 M1,
+| DOS.Sem.mkState s1 td1 ps1 ecs1 gl1 fs1 M1,
   NDOS.mkState s2 td2 ps2 ecs2 gl2 fs2 M2 =>
     s1 = s2 /\ td1 = td2 /\ ps1 = ps2 /\ instantiate_ECs ecs1 ecs2 /\ gl1 = gl2
     /\ fs1 = fs2 /\ M1 = M2
@@ -505,7 +504,7 @@ Qed.
 
 Lemma instantiate_locals__getOperandValue : forall TD v lc1 lc2 gl gvs1,
   instantiate_locals lc1 lc2 -> 
-  DOS.getOperandValue TD v lc1 gl = Some gvs1 ->
+  DOS.Sem.getOperandValue TD v lc1 gl = Some gvs1 ->
   exists gvs2, NDOS.getOperandValue TD v lc2 gl = Some gvs2 /\
     instantiate_gvs gvs1 gvs2.
 Proof.
@@ -513,7 +512,7 @@ Proof.
   destruct v; simpl in *.
     eapply instantiate_locals__lookup; eauto.
 
-    unfold DOS.const2GV in H0. unfold NDOS.const2GV.
+    unfold DOS.Sem.const2GV in H0. unfold NDOS.const2GV.
     destruct (_const2GV TD gl c) as [[gv ?]|]; inv H0.
     eauto using instantiate_gvs__cgv2gvs.
 Qed.
@@ -537,14 +536,14 @@ Lemma instantiate_locals__returnUpdateLocals : forall TD lc1 lc2 lc1' lc2' Resul
     gl lc1'' c,
   instantiate_locals lc1 lc2 -> 
   instantiate_locals lc1' lc2' -> 
-  DOS.returnUpdateLocals TD c Result lc1 lc1' gl = ret lc1'' ->
+  DOS.Sem.returnUpdateLocals TD c Result lc1 lc1' gl = ret lc1'' ->
   exists lc2'', 
     NDOS.returnUpdateLocals TD c Result lc2 lc2' gl = ret lc2'' /\
     instantiate_locals lc1'' lc2''. 
 Proof.
   intros.
-  unfold DOS.returnUpdateLocals in H1.
-  remember (DOS.getOperandValue TD Result lc1 gl) as R.
+  unfold DOS.Sem.returnUpdateLocals in H1.
+  remember (DOS.Sem.getOperandValue TD Result lc1 gl) as R.
   destruct R; tinv H1.
   symmetry in HeqR.
   eapply instantiate_locals__getOperandValue in HeqR; eauto.
@@ -564,7 +563,7 @@ Qed.
 
 Lemma instantiate_locals__getIncomingValuesForBlockFromPHINodes : forall TD b
     gl lc1 lc2 (Hlc : instantiate_locals lc1 lc2) ps re1,  
-  DOS.getIncomingValuesForBlockFromPHINodes TD ps b gl lc1 = Some re1 ->
+  DOS.Sem.getIncomingValuesForBlockFromPHINodes TD ps b gl lc1 = Some re1 ->
   exists re2,
     NDOS.getIncomingValuesForBlockFromPHINodes TD ps b gl lc2 = Some re2 /\
     instantiate_locals re1 re2.
@@ -574,12 +573,12 @@ Proof.
 
     destruct a.
     destruct (getValueViaBlockFromValuels l0 b); tinv H.
-    remember (DOS.getOperandValue TD v lc1 gl) as R.
+    remember (DOS.Sem.getOperandValue TD v lc1 gl) as R.
     destruct R; tinv H.
     symmetry in HeqR.  
     eapply instantiate_locals__getOperandValue in HeqR; eauto.
     destruct HeqR as [gvs2 [J1 J2]].
-    remember (DOS.getIncomingValuesForBlockFromPHINodes TD ps b gl lc1) as R1.
+    remember (DOS.Sem.getIncomingValuesForBlockFromPHINodes TD ps b gl lc1) as R1.
     destruct R1; inv H.  
     rewrite J1.
     symmetry in HeqR1.
@@ -591,7 +590,7 @@ Qed.
 Lemma instantiate_locals__updateValuesForNewBlock : forall lc1 lc2 re1 re2,
   instantiate_locals lc1 lc2 ->
   instantiate_locals re1 re2 ->
-  instantiate_locals (DOS.updateValuesForNewBlock re1 lc1)
+  instantiate_locals (DOS.Sem.updateValuesForNewBlock re1 lc1)
      (NDOS.updateValuesForNewBlock re2 lc2).
 Proof.
   induction re1; destruct re2; simpl; intros; auto.
@@ -603,18 +602,18 @@ Qed.
 
 Lemma instantiate_locals__switchToNewBasicBlock : forall TD lc1 lc2 gl lc1' b b',
   instantiate_locals lc1 lc2 -> 
-  DOS.switchToNewBasicBlock TD b' b gl lc1 = Some lc1' ->
+  DOS.Sem.switchToNewBasicBlock TD b' b gl lc1 = Some lc1' ->
   exists lc2', NDOS.switchToNewBasicBlock TD b' b gl lc2 = Some lc2' /\
     instantiate_locals lc1' lc2'. 
 Proof.
   intros.
-  unfold DOS.switchToNewBasicBlock in H0.
+  unfold DOS.Sem.switchToNewBasicBlock in H0.
   unfold NDOS.switchToNewBasicBlock.
-  remember (DOS.getIncomingValuesForBlockFromPHINodes TD 
+  remember (DOS.Sem.getIncomingValuesForBlockFromPHINodes TD 
     (getPHINodesFromBlock b') b gl lc1) as R.
   destruct R; inv H0.
   symmetry in HeqR.
-  eapply instantiate_locals__getIncomingValuesForBlockFromPHINodes in HeqR; eauto.
+  eapply instantiate_locals__getIncomingValuesForBlockFromPHINodes in HeqR;eauto.
   destruct HeqR as [re2 [J1 J2]].
   rewrite J1.
   eauto using instantiate_locals__updateValuesForNewBlock.
@@ -622,12 +621,12 @@ Qed.
 
 Lemma instantiate_locals__BOP : forall TD lc1 lc2 gl v1 v2 gvs3 bop sz,
   instantiate_locals lc1 lc2 -> 
-  DOS.BOP TD lc1 gl bop sz v1 v2 = Some gvs3 ->
+  DOS.Sem.BOP TD lc1 gl bop sz v1 v2 = Some gvs3 ->
   exists gvs3', NDOS.BOP TD lc2 gl bop sz v1 v2 = Some gvs3' /\
     instantiate_gvs gvs3 gvs3'.
 Proof.
   intros.
-  apply DOSprop.BOP_inversion in H0.
+  apply DOS.SemP.BOP_inversion in H0.
   destruct H0 as [gv1 [gv2 [J1 [J2 J3]]]]; subst.
   eapply instantiate_locals__getOperandValue in J1; eauto.
   destruct J1 as [gvs1 [H1 H2]].
@@ -640,12 +639,12 @@ Qed.
   
 Lemma instantiate_locals__FBOP : forall TD lc1 lc2 gl v1 v2 gv3 fbop fp,
   instantiate_locals lc1 lc2 -> 
-  DOS.FBOP TD lc1 gl fbop fp v1 v2 = Some gv3 ->
+  DOS.Sem.FBOP TD lc1 gl fbop fp v1 v2 = Some gv3 ->
   exists gvs3', NDOS.FBOP TD lc2 gl fbop fp v1 v2 = Some gvs3' /\
     instantiate_gvs gv3 gvs3'.
 Proof.
   intros.
-  apply DOSprop.FBOP_inversion in H0.
+  apply DOS.SemP.FBOP_inversion in H0.
   destruct H0 as [gv1 [gv2 [J1 [J2 J3]]]]; subst.
   eapply instantiate_locals__getOperandValue in J1; eauto.
   destruct J1 as [gvs1 [H1 H2]].
@@ -658,12 +657,12 @@ Qed.
 
 Lemma instantiate_locals__ICMP : forall TD lc1 lc2 gl v1 v2 gv3 c t,
   instantiate_locals lc1 lc2 -> 
-  DOS.ICMP TD lc1 gl c t v1 v2 = Some gv3 ->
+  DOS.Sem.ICMP TD lc1 gl c t v1 v2 = Some gv3 ->
   exists gvs3', NDOS.ICMP TD lc2 gl c t v1 v2 = Some gvs3' /\
     instantiate_gvs gv3 gvs3'.
 Proof.
   intros.
-  apply DOSprop.ICMP_inversion in H0.
+  apply DOS.SemP.ICMP_inversion in H0.
   destruct H0 as [gv1 [gv2 [J1 [J2 J3]]]]; subst.
   eapply instantiate_locals__getOperandValue in J1; eauto.
   destruct J1 as [gvs1 [H1 H2]].
@@ -676,12 +675,12 @@ Qed.
 
 Lemma instantiate_locals__FCMP : forall TD lc1 lc2 gl v1 v2 gv3 c t,
   instantiate_locals lc1 lc2 -> 
-  DOS.FCMP TD lc1 gl c t v1 v2 = Some gv3 ->
+  DOS.Sem.FCMP TD lc1 gl c t v1 v2 = Some gv3 ->
   exists gvs3', NDOS.FCMP TD lc2 gl c t v1 v2 = Some gvs3' /\
     instantiate_gvs gv3 gvs3'.
 Proof.
   intros.
-  apply DOSprop.FCMP_inversion in H0.
+  apply DOS.SemP.FCMP_inversion in H0.
   destruct H0 as [gv1 [gv2 [J1 [J2 J3]]]]; subst.
   eapply instantiate_locals__getOperandValue in J1; eauto.
   destruct J1 as [gvs1 [H1 H2]].
@@ -699,16 +698,16 @@ Hint Unfold instantiate_list_gvs.
 
 Lemma instantiate_locals__values2GVs : forall TD lc1 lc2 gl idxs vidxs,
   instantiate_locals lc1 lc2 -> 
-  DOS.values2GVs TD idxs lc1 gl = Some vidxs ->
+  DOS.Sem.values2GVs TD idxs lc1 gl = Some vidxs ->
   exists vidxss, NDOS.values2GVs TD idxs lc2 gl = Some vidxss /\
     instantiate_list_gvs vidxs vidxss.
 Proof.
   induction idxs; simpl; intros.
     inv H0. exists nil. auto.
 
-    remember (DOS.getOperandValue TD v lc1 gl) as R.
+    remember (DOS.Sem.getOperandValue TD v lc1 gl) as R.
     destruct R; tinv H0.
-    remember (DOS.values2GVs TD idxs lc1 gl) as R1.
+    remember (DOS.Sem.values2GVs TD idxs lc1 gl) as R1.
     destruct R1; inv H0.
     symmetry in HeqR.
     eapply instantiate_locals__getOperandValue in HeqR; eauto.
@@ -719,7 +718,7 @@ Qed.
 
 Lemma in_instantiate_list_gvs : forall vidxss1 vidxss2 vidxs1
   (Hinst1 : instantiate_list_gvs vidxss1 vidxss2)
-  (Hin1 : DOS.in_list_gvs vidxs1 vidxss1),
+  (Hin1 : DOS.Sem.in_list_gvs vidxs1 vidxss1),
   NDOS.in_list_gvs vidxs1 vidxss2.
 Proof.
   intros.
@@ -732,8 +731,8 @@ Lemma instantiate_locals__GEP : forall TD t mp1 mp1' vidxs1 vidxss1 vidxss2
     inbounds mps2,
   instantiate_list_gvs vidxss1 vidxss2 ->
   instantiate_gvs mp1 mps2 ->
-  DOS.in_list_gvs vidxs1 vidxss1 ->
-  DOS.GEP TD t mp1 vidxs1 inbounds = Some mp1' ->
+  DOS.Sem.in_list_gvs vidxs1 vidxss1 ->
+  DOS.Sem.GEP TD t mp1 vidxs1 inbounds = Some mp1' ->
   exists vidxs2, exists mps2', 
     NDOS.in_list_gvs vidxs2 vidxss2 /\
     NDOS.GEP TD t mps2 vidxs2 inbounds = Some mps2' /\ 
@@ -743,7 +742,7 @@ Proof.
     Hgep.
   inv Hgep.
   unfold NDOS.GEP.
-  unfold DOS.GEP in H0.
+  unfold DOS.Sem.GEP in H0.
   eapply instantiate_gvs__lift_op1 in H0; eauto.
   destruct H0 as [ys2 [J1 J2]].
   exists vidxs1.  
@@ -754,12 +753,12 @@ Lemma instantiate_locals__extractGenericValue : forall TD lc1 lc2 t gv2
     cidxs gv1 gvs1,
   instantiate_locals lc1 lc2 -> 
   instantiate_gvs gv1 gvs1 ->
-  DOS.extractGenericValue TD t gv1 cidxs = Some gv2 ->
+  DOS.Sem.extractGenericValue TD t gv1 cidxs = Some gv2 ->
   exists gvs2, NDOS.extractGenericValue TD t gvs1 cidxs = Some gvs2 
     /\ instantiate_gvs gv2 gvs2.
 Proof.
   intros.
-  unfold DOS.extractGenericValue in H1.
+  unfold DOS.Sem.extractGenericValue in H1.
   unfold NDOS.extractGenericValue.
   destruct (intConsts2Nats TD cidxs); inv H1.
   destruct (mgetoffset TD t l0) as [[]|]; inv H3.
@@ -771,12 +770,12 @@ Lemma instantiate_locals__insertGenericValue : forall TD lc1 lc2 t1 t2 gv2
   instantiate_locals lc1 lc2 -> 
   instantiate_gvs gv1 gvs1 ->
   instantiate_gvs gv2 gvs2 ->
-  DOS.insertGenericValue TD t1 gv1 cidxs t2 gv2 = Some gv3 ->
+  DOS.Sem.insertGenericValue TD t1 gv1 cidxs t2 gv2 = Some gv3 ->
   exists gvs3, NDOS.insertGenericValue TD t1 gvs1 cidxs t2 gvs2 = Some gvs3
     /\ instantiate_gvs gv3 gvs3.
 Proof.
   intros.
-  unfold DOS.insertGenericValue in H2.
+  unfold DOS.Sem.insertGenericValue in H2.
   unfold NDOS.insertGenericValue.
   destruct (intConsts2Nats TD cidxs); inv H2.
   destruct (mgetoffset TD t1 l0) as [[]|]; inv H4.
@@ -785,12 +784,12 @@ Qed.
 
 Lemma instantiate_locals__CAST : forall TD lc1 lc2 gl t1 v1 t2 gv2 castop0,
   instantiate_locals lc1 lc2 -> 
-  DOS.CAST TD lc1 gl castop0 t1 v1 t2 = Some gv2 ->
+  DOS.Sem.CAST TD lc1 gl castop0 t1 v1 t2 = Some gv2 ->
   exists gvs2', NDOS.CAST TD lc2 gl castop0 t1 v1 t2 = Some gvs2' 
     /\ instantiate_gvs gv2 gvs2'.
 Proof.
   intros.
-  apply DOSprop.CAST_inversion in H0.
+  apply DOS.SemP.CAST_inversion in H0.
   destruct H0 as [gv1 [J1 J2]]; subst.
   eapply instantiate_locals__getOperandValue in J1; eauto.
   destruct J1 as [gvs1 [H1 H2]].
@@ -801,12 +800,12 @@ Qed.
 
 Lemma instantiate_locals__TRUNC : forall TD lc1 lc2 gl t1 v1 t2 gv2 top0,
   instantiate_locals lc1 lc2 -> 
-  DOS.TRUNC TD lc1 gl top0 t1 v1 t2 = Some gv2 ->
+  DOS.Sem.TRUNC TD lc1 gl top0 t1 v1 t2 = Some gv2 ->
   exists gvs2', NDOS.TRUNC TD lc2 gl top0 t1 v1 t2 = Some gvs2' 
     /\ instantiate_gvs gv2 gvs2'.
 Proof.
   intros.
-  apply DOSprop.TRUNC_inversion in H0.
+  apply DOS.SemP.TRUNC_inversion in H0.
   destruct H0 as [gv1 [J1 J2]]; subst.
   eapply instantiate_locals__getOperandValue in J1; eauto.
   destruct J1 as [gvs1 [H1 H2]].
@@ -817,12 +816,12 @@ Qed.
 
 Lemma instantiate_locals__EXT : forall TD lc1 lc2 gl t1 v1 t2 gv2 top0,
   instantiate_locals lc1 lc2 -> 
-  DOS.EXT TD lc1 gl top0 t1 v1 t2 = Some gv2 ->
+  DOS.Sem.EXT TD lc1 gl top0 t1 v1 t2 = Some gv2 ->
   exists gvs2', NDOS.EXT TD lc2 gl top0 t1 v1 t2 = Some gvs2' 
     /\ instantiate_gvs gv2 gvs2'.
 Proof.
   intros.
-  apply DOSprop.EXT_inversion in H0.
+  apply DOS.SemP.EXT_inversion in H0.
   destruct H0 as [gv1 [J1 J2]]; subst.
   eapply instantiate_locals__getOperandValue in J1; eauto.
   destruct J1 as [gvs1 [H1 H2]].
@@ -833,7 +832,7 @@ Qed.
 
 Lemma instantiate_locals__params2GVs : forall TD lc1 lc2 gl 
   (Hlc:instantiate_locals lc1 lc2) lp gvs1,
-  DOS.params2GVs TD lp lc1 gl = Some gvs1 ->
+  DOS.Sem.params2GVs TD lp lc1 gl = Some gvs1 ->
   exists gvss2, NDOS.params2GVs TD lp lc2 gl = Some gvss2 /\
     instantiate_list_gvs gvs1 gvss2.
 Proof.
@@ -841,9 +840,9 @@ Proof.
     inv H. eauto.
 
     destruct a.
-    remember (DOS.getOperandValue TD v lc1 gl) as R1.
+    remember (DOS.Sem.getOperandValue TD v lc1 gl) as R1.
     destruct R1; tinv H.
-    remember (DOS.params2GVs TD lp lc1 gl) as R2.
+    remember (DOS.Sem.params2GVs TD lp lc1 gl) as R2.
     destruct R2; inv H.
     symmetry in HeqR1.
     eapply instantiate_locals__getOperandValue in HeqR1; eauto.
@@ -855,7 +854,7 @@ Qed.
 Lemma instantiate_locals__initializeFrameValues : forall TD lc1 lc2
   (H2: instantiate_locals lc1 lc2) la gvs1 gvs2 lc1'
   (H1 : instantiate_list_gvs gvs1 gvs2),
-  DOS._initializeFrameValues TD la gvs1 lc1 = Some lc1' ->
+  DOS.Sem._initializeFrameValues TD la gvs1 lc1 = Some lc1' ->
   exists lc2',
     NDOS._initializeFrameValues TD la gvs2 lc2 = Some lc2' /\
     instantiate_locals lc1' lc2'.
@@ -866,7 +865,7 @@ Proof.
     destruct a. destruct p.
     destruct gvs1; simpl.
       destruct gvs2; inv H1.
-      remember (DOS._initializeFrameValues TD la nil lc1) as R1.
+      remember (DOS.Sem._initializeFrameValues TD la nil lc1) as R1.
       destruct R1; tinv H.
       destruct (gundef TD t); inv H.
       symmetry in HeqR1.
@@ -878,7 +877,7 @@ Proof.
 
       simpl in H1.
       destruct gvs2; inv H1.
-      remember (DOS._initializeFrameValues TD la gvs1 lc1) as R1.
+      remember (DOS.Sem._initializeFrameValues TD la gvs1 lc1) as R1.
       destruct R1; tinv H.
       remember (DGVs.lift_op1 (fit_gv TD t) t0 t) as R2.
       destruct R2; inv H.
@@ -895,12 +894,12 @@ Qed.
 
 Lemma instantiate_locals__initLocals : forall TD gvs1 gvss2 
   (H : instantiate_list_gvs gvs1 gvss2) la lc1,
-  DOS.initLocals TD la gvs1 = Some lc1 ->
+  DOS.Sem.initLocals TD la gvs1 = Some lc1 ->
   exists lc2, 
     NDOS.initLocals TD la gvss2 = Some lc2 /\
     instantiate_locals lc1 lc2.
 Proof.
-  unfold DOS.initLocals, NDOS.initLocals.
+  unfold DOS.Sem.initLocals, NDOS.initLocals.
   intros.
   eapply instantiate_locals__initializeFrameValues; eauto.
     simpl. auto.
@@ -908,7 +907,7 @@ Qed.
 
 Lemma instantiate_list_gvs__incl : forall x y x0,
   instantiate_list_gvs x y ->
-  DOS.in_list_gvs x0 x ->
+  DOS.Sem.in_list_gvs x0 x ->
   NDOS.in_list_gvs x0 y.
 Proof.
   intros.  
@@ -922,13 +921,13 @@ Qed.
 Lemma instantiate_locals__exCallUpdateLocals : forall TD lc1 lc2 lc1' rid oResult
     nr ft,
   instantiate_locals lc1 lc2 -> 
-  DOS.exCallUpdateLocals TD ft nr rid oResult lc1 = ret lc1' ->
+  DOS.Sem.exCallUpdateLocals TD ft nr rid oResult lc1 = ret lc1' ->
   exists lc2', 
     NDOS.exCallUpdateLocals TD ft nr rid oResult lc2 = ret lc2' /\
     instantiate_locals lc1' lc2'. 
 Proof.
   intros.
-  unfold DOS.exCallUpdateLocals in H0.
+  unfold DOS.Sem.exCallUpdateLocals in H0.
   unfold NDOS.exCallUpdateLocals.
   destruct nr; inv H0; eauto.
   destruct oResult; inv H2; eauto.
@@ -940,7 +939,7 @@ Qed.
 
 Ltac simpl_nd_llvmds :=
   match goal with
-  | [Hsim : instantiate_State {| DOS.ECS := _::_::_ |} ?st2 |- _ ] =>
+  | [Hsim : instantiate_State {| DOS.Sem.ECS := _::_::_ |} ?st2 |- _ ] =>
      destruct st2 as [S' TD' Ps' ECs' gl' fs' M'];
      destruct Hsim as [eq1 [eq2 [eq3 [Hsim [eq4 [eq5 eq6]]]]]]; subst;
      destruct ECs' as [|[f1' b1' cs1' tmn1' lc1' als1'] ECs']; 
@@ -951,7 +950,7 @@ Ltac simpl_nd_llvmds :=
      destruct Hsim2 as [Hsim2 Hsim3];
      destruct Hsim1 as [J1 [J2 [J3 [J4 [Hsim1 J6]]]]]; subst;
      destruct Hsim2 as [J1 [J2 [J3 [J4 [Hsim2 J6]]]]]; subst
-  | [Hsim : instantiate_State {| DOS.ECS := _::_|} ?st2 |- _ ] =>
+  | [Hsim : instantiate_State {| DOS.Sem.ECS := _::_|} ?st2 |- _ ] =>
      destruct st2 as [S' TD' Ps' ECs' gl' fs' M'];
      destruct Hsim as [eq1 [eq2 [eq3 [Hsim [eq4 [eq5 eq6]]]]]]; subst;
      destruct ECs' as [|[f1' b1' cs1' tmn1' lc1' als1'] ECs']; 
@@ -962,7 +961,7 @@ Ltac simpl_nd_llvmds :=
 
 Lemma instantiate_dsInsn : forall st1 st2 st1' tr,
   instantiate_State st1 st2 ->
-  DOS.sInsn st1 st1' tr ->
+  DOS.Sem.sInsn st1 st1' tr ->
   (exists st2', NDOS.sInsn st2 st2' tr /\ instantiate_State st1' st2').
 Proof.
   intros st1 st2 st1' tr Hsim Hop.  
